

LECTURE 18 - EQUATIONS OF MOTION - MDOF SYSTEMS - PART II

CE 225

Prof DeJong

UC Berkeley

October 30, 2025

EXAMPLE 1: LUMPED MASS WITH ROTATIONAL INERTIA

EXAMPLE 1: LUMPED MASS WITH ROTATIONAL INERTIA

(CONTINUED)

$$\underline{\underline{k}} = \frac{EI}{h^3} \begin{bmatrix} 12 & 6h \\ 6h & 4h^2 \end{bmatrix} \quad \underline{\underline{m}} = \begin{bmatrix} m & 0 \\ 0 & J \end{bmatrix}$$

EXAMPLE 2: BEAM WITH POINT MASSES

Use 'Stiffness Method' to derive EOM.

Deflection at tip:

$$u_1 = \frac{f_{11}L^3}{3EI} + \left[\frac{f_{21}(L/2)^3}{3EI} + \frac{f_{21}(L/2)^2}{2EI} \frac{L}{2} \right] = 1 \quad (1)$$

Deflection at midspan:

$$u_2 = \frac{f_{21}(L/2)^3}{3EI} + \frac{f_{11}(L/2)^3}{3EI} + \frac{\left(f_{11}\frac{L}{2}\right)(L/2)^2}{2EI} = 0 \quad (2)$$

EXAMPLE 2: BEAM WITH POINT MASSES

Solve (1) and (2) simultaneously
$$\begin{cases} f_{11} = k_{11} = \frac{48}{7} \frac{2EI}{L^3} \\ f_{21} = k_{21} = \frac{48}{7} \left(\frac{-5EI}{L^3} \right) \end{cases}$$

Deflection at tip:
$$u_1 = \frac{f_{12}L^3}{3EI} + \left[\frac{f_{22}(L/2)^3}{3EI} + \frac{f_{12}(L/2)^2}{2EI} \frac{L}{2} \right] = 0$$

$$\longrightarrow f_{22} = k_{22} = \frac{48}{7} \frac{16EI}{L^3}$$

Therefore, EOM:

$$\boxed{\begin{bmatrix} mL/4 & 0 \\ 0 & mL/2 \end{bmatrix} \ddot{\underline{u}} + \frac{48}{7} \frac{EI}{L^3} \begin{bmatrix} 2 & -5 \\ -5 & 16 \end{bmatrix} \underline{u} = \begin{bmatrix} p_1(t) \\ p_2(t) \end{bmatrix}}$$

FLEXIBILITY METHOD

Theory:

$$\begin{bmatrix} u_1 \\ u_2 \\ \vdots \\ u_N \end{bmatrix} = \begin{bmatrix} \hat{f}_{11} & \hat{f}_{12} & \cdots & \hat{f}_{1N} \\ \hat{f}_{21} & \hat{f}_{22} & \cdots & \hat{f}_{2N} \\ \vdots & \vdots & \ddots & \vdots \\ \hat{f}_{N1} & \hat{f}_{N2} & \cdots & \hat{f}_{NN} \end{bmatrix} \begin{bmatrix} f_1 \\ f_2 \\ \vdots \\ f_N \end{bmatrix} \longrightarrow \underline{u} = \underline{\hat{f}} \underline{f} \longrightarrow \underline{\hat{f}} = \underline{k}^{-1}$$

If $f_1 = 1$ and all other forces are zero \longrightarrow

$$\begin{bmatrix} u_1 \\ u_2 \\ \vdots \\ u_N \end{bmatrix} = \begin{bmatrix} \hat{f}_{11} \\ \hat{f}_{21} \\ \vdots \\ \hat{f}_{N1} \end{bmatrix}$$

**Therefore, the displacements that result from the forces $f_1 = 1$ and $f_2 = f_3 = \dots = f_N = 0$ actually provide the first column of the flexibility matrix $\underline{\hat{f}}$

Then repeat for other DOFs.

FLEXIBILITY METHOD

EXAMPLE 2 (AGAIN)

$$f_1 = 1 \quad f_2 = 0$$

$$f_{11} = \frac{1L^3}{3EI}$$
$$f_{21} = \frac{(L/2)^3}{3EI} + \frac{(L/2)(L/2)^2}{2EI} = \frac{5}{48} \frac{L^3}{EI}$$

$$f_1 = 0 \quad f_2 = 1$$

$$f_{22} = \frac{(L/2)^3}{3EI} = \frac{2L^3}{48EI}$$

$$\underline{\underline{f}} = \frac{L^3}{48EI} \begin{bmatrix} 16 & 5 \\ 5 & 2 \end{bmatrix} \longrightarrow \text{Now, } \underline{\underline{k}} = \underline{\underline{f}}^{-1} \text{ yields same as before!}$$

MORE GENERALIZED APPROACH (STATIC CONDENSATION)

EXAMPLE 2 (THIRD TIME)

The equation of motion is given by:

$$\begin{bmatrix} m\frac{L}{4} & 0 & 0 & 0 \\ 0 & m\frac{L}{2} & 0 & 0 \\ 0 & 0 & 0 & 0 \\ 0 & 0 & 0 & 0 \end{bmatrix} \ddot{\underline{u}} + \frac{8EI}{L^3} \begin{bmatrix} 12 & -12 & -3L & -3L \\ -12 & 24 & 3L & 0 \\ -3L & 3L & L^2 & \frac{L^2}{2} \\ -3L & 0 & \frac{L^2}{2} & L^2 \end{bmatrix} \underline{u} = \begin{bmatrix} p_1 \\ p_2 \\ 0 \\ 0 \end{bmatrix}$$

However, we have more DOF's than are needed (only two masses!).

MORE GENERALIZED APPROACH (STATIC CONDENSATION)

EXAMPLE 2 (THIRD TIME)

Rewrite EOMs in the following form:

$$\begin{bmatrix} \underline{m}_{tt} & \underline{0} \\ \underline{0} & \underline{0} \end{bmatrix} \begin{bmatrix} \ddot{\underline{u}}_t \\ \ddot{\underline{u}}_0 \end{bmatrix} + \begin{bmatrix} \underline{k}_{tt} & \underline{k}_{t0} \\ \underline{k}_{0t} & \underline{k}_{00} \end{bmatrix} \begin{bmatrix} \underline{u}_t \\ \underline{u}_0 \end{bmatrix} = \begin{bmatrix} \underline{p}_t \\ \underline{p}_0 \end{bmatrix}$$

Write 2 separate equations in the following form:

$$\underline{m}_{tt}\ddot{\underline{u}}_t + \underline{k}_{tt}\underline{u}_t + \underline{k}_{t0}\underline{u}_0 = \underline{p}_t$$

$$\underline{k}_{0t}\underline{u}_t + \underline{k}_{00}\underline{u}_0 = \underline{0} \quad \longrightarrow \quad \boxed{\underline{u}_0 = -\underline{k}_{00}^{-1}\underline{k}_{0t}\underline{u}_t}$$

Plug \underline{u}_0 into first equation: $\underline{m}_{tt}\ddot{\underline{u}}_t + \underline{k}_{tt}\underline{u}_t + \underline{k}_{t0}[-\underline{k}_{00}^{-1}\underline{k}_{0t}\underline{u}_t] = \underline{p}_t$

Rearrange: $\underline{m}_{tt}\ddot{\underline{u}}_t + [\underline{k}_{tt} - \underline{k}_{t0}^T \underline{k}_{00}^{-1} \underline{k}_{0t}] \underline{u}_t = \underline{p}_t \quad \longrightarrow \quad \text{Note: } [\underline{k}_{tt} - \underline{k}_{t0}^T \underline{k}_{00}^{-1} \underline{k}_{0t}] = \frac{48 EI}{7 L^3} \begin{bmatrix} 2 & -5 \\ -5 & 16 \end{bmatrix}$

REVIEW